ROOT
@@ -1926,6 +1926,7 @@ session RRA_Factor_Structural_Bootstrap = HOL +
     Development_Given_Installed_Declarations
     Development_Installed_Presentations_Execution
     Development_First_Problem_Asked
+    Development_Socket_Liveness_Execution
     Development_Asked_Registrations
     Development_First_Request_Program
     Development_First_Request_Registrations
